Added a procedure Hoare triple, which introduces a variable for the return value. Removed this syntax for ghost variables.

UTP/ITree_Procedure.thy
@@ -5,19 +5,43 @@ theory ITree_Procedure
   keywords "over"
 begin
 
-definition "rbind x = (\<lambda> (r, s). Ret (put\<^bsub>x\<^esub> s r))"
+subsection \<open> Modelling Procedures \<close>
 
-definition "rdrop = (\<lambda> (r, s). Ret s)"
+text \<open> Procedures are implemented by having heterogeneous ITrees with a pair return type 
+  @{typ "'a \<times> 's"}, where @{typ "'s"} is the state and @{typ "'a"} is the return type. The
+  following type models a procedure with input @{typ "'a"}, return type @{typ "'r"}, 
+  and state type @{typ "'s"}. \<close>
+
+type_synonym ('a, 'r, 's, 'e) iproc = "'a \<Rightarrow> 's \<Rightarrow> ('e, 'r \<times> 's) itree"
+
+subsection \<open> Constructors \<close>
+
+text \<open> Bind a return value to a lens \<close>
+
+definition rbind :: "('a \<Longrightarrow> 's) \<Rightarrow> 'a \<times> 's \<Rightarrow> ('e, 's) itree" where 
+"rbind x = (\<lambda> (r, s). Ret (put\<^bsub>x\<^esub> s r))"
+
+text \<open> Drop a return value \<close>
+
+definition rdrop :: "'a \<times> 's \<Rightarrow> ('e, 's) itree" where
+"rdrop = (\<lambda> (r, s). Ret s)"
+
+text \<open> Call a procedure with a variable to store the return value, and expression to provide
+  the inputs. \<close>
 
 definition proc_call :: 
-  "('r \<Longrightarrow> 's) \<Rightarrow> ('a \<Rightarrow> 's \<Rightarrow> ('e, 'r \<times> 's) itree) \<Rightarrow> ('a, 's) expr \<Rightarrow> ('e, 's) htree" where
+  "('r \<Longrightarrow> 's) \<Rightarrow> ('a, 'r, 's, 'e) iproc \<Rightarrow> ('a, 's) expr \<Rightarrow> ('e, 's) htree" where
 [code_unfold]: 
   "proc_call x pr prm = (\<lambda> s. pr (prm s) s \<bind> rbind x)"
+
+text \<open> Call a procedure without binding the return value. \<close>
 
 definition proc_call_nret :: 
   "('a \<Rightarrow> 's \<Rightarrow> ('e, 'r \<times> 's) itree) \<Rightarrow> ('a, 's) expr \<Rightarrow> ('e, 's) htree" where
   [code_unfold]: 
   "proc_call_nret pr prm = (\<lambda> s. pr (prm s) s \<bind> rdrop)"
+
+text \<open> Return statements in an ITree procedure \<close>
 
 definition proc_ret :: "('s \<Rightarrow> 'a) \<Rightarrow> 's \<Rightarrow> ('e, 'a \<times> 's) itree" where 
   "proc_ret e = (\<lambda> s. Ret (e s, s))"
@@ -37,6 +61,8 @@ lemma ret_drop [simp]: "proc_ret e ;; rdrop = Skip"
 lemma ret_drop' [simp]: "(P ;; proc_ret e) ;; rdrop = P"
   by (simp add: kcomp_assoc)
 
+subsection \<open> Syntax \<close>
+
 syntax 
   "_call"      :: "svid \<Rightarrow> id \<Rightarrow> logic \<Rightarrow> logic" ("_ := <_ _>" [61, 0, 61] 61)
   "_call_nret" :: "id \<Rightarrow> logic \<Rightarrow> logic" ("call _ _" [0, 61] 61) 
@@ -46,6 +72,40 @@ translations
   "_return e" == "CONST proc_ret (e)\<^sub>e"
   "_call x P e" == "CONST proc_call x P (e)\<^sub>e"
   "_call_nret P e" == "CONST proc_call_nret P (e)\<^sub>e"
+
+ML_file \<open>ITree_Procedure.ML\<close>
+
+subsection \<open> Hoare logic \<close>
+
+text \<open> We implement a specialised form of Hoare triple, which accepts a procedure as the program.
+  The postcondition introduces a variable, to which the return value of the procedure is bound.
+  Otherwise, the postcondition is the same as a normal Hoare triple. \<close>
+
+definition hoare_rel_proc_triple :: "('s \<Rightarrow> bool) \<Rightarrow> ('s \<Rightarrow> ('e, 'a \<times> 's) itree) \<Rightarrow> ('a \<Rightarrow> 's \<Rightarrow> 's \<Rightarrow> bool) \<Rightarrow> bool" where
+"hoare_rel_proc_triple P C Q = (\<forall> s s' r es. P s \<and> C s \<midarrow>es\<leadsto> \<checkmark> (r, s') \<longrightarrow> Q r s s')"
+
+syntax   
+  "_hoare_proc" :: "logic \<Rightarrow> logic \<Rightarrow> id \<Rightarrow> logic \<Rightarrow> logic" ("(2H{_} /_) /{_./ _}")
+
+translations
+  "H{P} C {x. Q}" => "CONST hoare_rel_proc_triple (P)\<^sub>e C (\<lambda> x _ghost_old. (Q)\<^sub>e)"
+  "H{P} C {x. Q}" <= "CONST hoare_rel_proc_triple (P)\<^sub>e C (\<lambda> x g. (Q)\<^sub>e)"
+
+lemma hl_return: 
+  "H{P} return e {ret. \<guillemotleft>ret\<guillemotright> = e \<and> P}"
+  by (simp add: hoare_rel_proc_triple_def proc_ret_def)
+
+lemma hl_proc_seq:
+  assumes "H{P} C\<^sub>1 {Q}" "H{Q} C\<^sub>2 {ret. @(R ret)}"
+  shows "H{P} C\<^sub>1 ;; C\<^sub>2 {ret. @(R ret)}"
+  using assms
+  by (auto elim!:trace_to_bindE bind_RetE' simp add: hoare_rel_proc_triple_def hoare_rel_triple_def seq_itree_def kleisli_comp_def)
+     (metis trace_to_Nil)+
+
+lemma hl_proc_seq_return [hoare_safe]:
+  assumes "H{P} C {Q}"
+  shows "H{P} C ;; return e {ret. \<guillemotleft>ret\<guillemotright> = e \<and> Q}"
+  using assms hl_proc_seq hl_return by fastforce
 
 lemma hl_proc_call [hoare_safe]: 
   assumes "\<And> v. H{P \<and> \<guillemotleft>v\<guillemotright> = e} C(v) ;; rbind x {Q}"
@@ -76,7 +136,5 @@ lemma thl_proc_call_nret [hoare_safe]:
   apply (auto simp add: proc_call_nret_def taut_def seq_itree_def kleisli_comp_def)
   apply (metis (mono_tags, lifting) SEXP_def kleisli_comp_def pre_terminates seq_itree_def wp_seq)
   done
-
-ML_file \<open>ITree_Procedure.ML\<close>
 
 end
